Flip ordinal multiplication’s arguments.
The argument that is recursed on is the second argument.  This gives

  2 × ω = ω ≠ ω + ω = ω × 2

This brings my notation in line with convention, as determined by
looking at

  Johnstone, “Notes on logic and set theory”
  Mendelson, “Intro. to mathematical logic”
  Potter, “Set theory and its philosophy”

and even Wikipedia.

examples/set-theory/hol_sets/ordinalScript.sml
@@ -1111,44 +1111,43 @@ val ordMULT_def = new_specification(
   "ordMULT_def", ["ordMULT"],
   ord_RECURSION |> INST_TYPE [beta |-> ``:'a ordinal``]
                 |> Q.SPEC `0`
-                |> Q.SPEC `λap r. r + b`
+                |> Q.SPEC `λap r. r + β`
                 |> Q.SPEC `λa preds. sup preds`
-                |> Q.GEN `b`
+                |> Q.GEN `β`
                 |> CONV_RULE SKOLEM_CONV
-                |> BETA_RULE
-                |> SIMP_RULE (srw_ss()) [Once exists_C]
-                |> SIMP_RULE (srw_ss()) [combinTheory.C_DEF])
+                |> BETA_RULE)
 val _ = export_rewrites ["ordMULT_def"]
 val _ = overload_on ("*", ``ordMULT``)
 
-val ordMULT_0R = store_thm(
-  "ordMULT_0R",
-  ``∀a:'a ordinal. a * 0 = 0``,
+val ordMULT_0L = store_thm(
+  "ordMULT_0L",
+  ``∀a:'a ordinal. 0 * a = 0``,
   ho_match_mp_tac simple_ord_induction >> simp[] >> qx_gen_tac `a` >>
-  strip_tac >> qsuff_tac `IMAGE (λy. y * 0) (preds a) = {0}` >> simp[] >>
-  simp[EXTENSION] >>
-  asm_simp_tac (srw_ss() ++ DNF_ss ++ CONJ_ss) [] >> metis_tac[]);
-val _ = export_rewrites ["ordMULT_0R"]
+  strip_tac >> qsuff_tac `IMAGE ($* 0) (preds a) = {0}` >> simp[] >>
+  simp[EXTENSION] >> metis_tac[]);
+val _ = export_rewrites ["ordMULT_0L"]
+
+val ordMULT_0R = store_thm("ordMULT_0R", ``∀a:'a ordinal. a * 0 = 0``, simp[]);
 
 val ordMULT_1L = store_thm(
   "ordMULT_1L",
-  ``1 * (a:'a ordinal) = a``,
-  REWRITE_TAC [GSYM ORD_ONE] >> simp[]);
+  ``∀a. 1 * (a:'a ordinal) = a``,
+  ho_match_mp_tac simple_ord_induction >> simp[ADD1R] >> qx_gen_tac `a` >>
+  strip_tac >> qsuff_tac `IMAGE ($* 1) (preds a) = preds a`
+  >- fs [sup_preds_omax_NONE] >>
+  dsimp[EXTENSION] >> asm_simp_tac (srw_ss() ++ CONJ_ss) []);
 val _ = export_rewrites ["ordMULT_1L"]
-
-val ordMULT_2L = store_thm(
-  "ordMULT_2L",
-  ``2 * (a:'a ordinal) = a + a``,
-  `2 = 1⁺` by simp[] >> pop_assum SUBST1_TAC >> simp[]);
 
 val ordMULT_1R = store_thm(
   "ordMULT_1R",
   ``∀a:'a ordinal. a * 1 = a``,
-  ho_match_mp_tac simple_ord_induction >> simp[ADD1R] >>
-  qx_gen_tac `a` >> strip_tac >>
-  qsuff_tac `IMAGE (λy. y * 1) (preds a) = preds a`
-  >- fs[sup_preds_omax_NONE] >>
-  dsimp[EXTENSION] >> asm_simp_tac (srw_ss() ++ CONJ_ss) []);
+  simp_tac bool_ss [GSYM ORD_ONE, ordMULT_def, ordADD_0L]);
+val _ = export_rewrites ["ordMULT_1R"]
+
+val ordMULT_2R = store_thm(
+  "ordMULT_2R",
+  ``(a:'a ordinal) * 2 = a + a``,
+  `2 = 1⁺` by simp[] >> pop_assum SUBST1_TAC >> simp[]);
 
 val ord_CASES = store_thm(
   "ord_CASES",
@@ -1163,100 +1162,100 @@ val islimit_SUC_lt = store_thm(
   ``islimit b ∧ a < b ⇒ a⁺ < b``,
   fs[omax_NONE] >> metis_tac [ordlt_SUC_DISCRETE, ordlt_trichotomy, ordle_lteq])
 
-val ordMULT_lt_MONO_L = store_thm(
-  "ordMULT_lt_MONO_L",
-  ``∀a b c:'a ordinal. a < b ∧ 0 < c ⇒ a * c < b * c``,
-  qsuff_tac `∀b a c:'a ordinal. a < b ∧ 0 < c ⇒ a * c < b * c` >- metis_tac[]>>
+val ordMULT_lt_MONO_R = store_thm(
+  "ordMULT_lt_MONO_R",
+  ``∀a b c:'a ordinal. a < b ∧ 0 < c ⇒ c * a < c * b``,
+  qsuff_tac `∀b a c:'a ordinal. a < b ∧ 0 < c ⇒ c * a < c * b` >- metis_tac[]>>
   ho_match_mp_tac simple_ord_induction >> simp[] >> conj_tac
   >- (simp[ordlt_SUC_DISCRETE] >> qx_gen_tac `b` >> strip_tac >>
       map_every qx_gen_tac [`a`, `c`] >>
       Cases_on `a = b` >> simp[] >> strip_tac >>
-      `a * c < b * c` by metis_tac[] >>
-      `b * c < b * c + c` by simp[] >> metis_tac [ordlt_TRANS]) >>
+      `c * a < c * b` by metis_tac[] >>
+      `c * b < c * b + c` by simp[] >> metis_tac [ordlt_TRANS]) >>
   qx_gen_tac `b` >> strip_tac >> map_every qx_gen_tac [`a`, `c`] >>
   strip_tac >> simp[predimage_sup_thm] >>
   `∃d. a < d ∧ d < b`
     by metis_tac[sup_preds_omax_NONE, IN_preds, preds_inj_univ, sup_thm] >>
   metis_tac[]);
 
-val ordMULT_le_MONO_L = store_thm(
-  "ordMULT_le_MONO_L",
-  ``∀a b c:'a ordinal. a ≤ b ⇒ a * c ≤ b * c``,
+val ordMULT_le_MONO_R = store_thm(
+  "ordMULT_le_MONO_R",
+  ``∀a b c:'a ordinal. a ≤ b ⇒ c * a ≤ c * b``,
   simp[ordle_lteq] >> rpt strip_tac >> simp[] >>
   Cases_on `c = 0` >> simp[] >>
   `0 < c` by metis_tac [ordlt_ZERO, ordlt_trichotomy] >>
-  metis_tac [ordMULT_lt_MONO_L])
+  metis_tac [ordMULT_lt_MONO_R])
 
-val ordMULT_lt_MONO_L_EQN = store_thm(
-  "ordMULT_lt_MONO_L_EQN",
-  ``a * c < b * c <=> a < b ∧ 0 < c``,
-  simp[EQ_IMP_THM, ordMULT_lt_MONO_L] >>
-  Cases_on `0 < c` >- metis_tac [ordMULT_le_MONO_L] >> fs[]);
-val _ = export_rewrites ["ordMULT_lt_MONO_L_EQN"]
+val ordMULT_lt_MONO_R_EQN = store_thm(
+  "ordMULT_lt_MONO_R_EQN",
+  ``c * a < c * b <=> a < b ∧ 0 < c``,
+  simp[EQ_IMP_THM, ordMULT_lt_MONO_R] >>
+  Cases_on `0 < c` >- metis_tac [ordMULT_le_MONO_R] >> fs[]);
+val _ = export_rewrites ["ordMULT_lt_MONO_R_EQN"]
 
 val ordADD_le_MONO_L = store_thm(
   "ordADD_le_MONO_L",
   ``x ≤ y ⇒ x + z ≤ y + z``,
   simp[ordle_lteq, SimpL ``$==>``] >> simp[DISJ_IMP_THM, ordADD_weak_MONO]);
 
-val ordMULT_le_MONO_R = store_thm(
-  "ordMULT_le_MONO_R",
-  ``∀a b c:'a ordinal. a ≤ b ⇒ c * a ≤ c * b``,
-  qsuff_tac `∀c a b:'a ordinal. a ≤ b ⇒ c * a ≤ c * b` >- metis_tac[] >>
+val ordMULT_le_MONO_L = store_thm(
+  "ordMULT_le_MONO_L",
+  ``∀a b c:'a ordinal. a ≤ b ⇒ a * c ≤ b * c``,
+  qsuff_tac `∀c a b:'a ordinal. a ≤ b ⇒ a * c ≤ b * c` >- metis_tac[] >>
   ho_match_mp_tac simple_ord_induction >> simp[] >> conj_tac
   >- (qx_gen_tac `c` >> strip_tac >> map_every qx_gen_tac [`a`, `b`] >>
       strip_tac >>
-      `c * a + a ≤ c * a + b` by simp[] >>
-      match_mp_tac ordle_TRANS >> qexists_tac `c * a + b` >> simp[] >>
+      `a * c + a ≤ a * c + b` by simp[] >>
+      match_mp_tac ordle_TRANS >> qexists_tac `a * c + b` >> simp[] >>
       simp[ordADD_le_MONO_L]) >>
   qx_gen_tac `c` >> strip_tac >> map_every qx_gen_tac [`a`, `b`] >> strip_tac>>
   simp[predimage_sup_thm, impI] >> qx_gen_tac `d` >> strip_tac >>
-  match_mp_tac ordle_TRANS >> qexists_tac `d * b` >> simp[] >>
-  qsuff_tac `d * b ∈ IMAGE (λy. y * b) (preds c)`
+  match_mp_tac ordle_TRANS >> qexists_tac `b * d` >> simp[] >>
+  qsuff_tac `b * d ∈ IMAGE ($* b) (preds c)`
   >- metis_tac [mklesup sup_thm, IMAGE_cardleq_rwt, preds_inj_univ] >>
   simp[] >> metis_tac[]);
 
-val ordMULT_CANCEL_L = store_thm(
-  "ordMULT_CANCEL_L",
-  ``(x * z = y * z:'a ordinal) <=> (z = 0) ∨ (x = y)``,
+val ordMULT_CANCEL_R = store_thm(
+  "ordMULT_CANCEL_R",
+  ``(z * x = z * y:'a ordinal) <=> (z = 0) ∨ (x = y)``,
   simp[EQ_IMP_THM, DISJ_IMP_THM] >> strip_tac >>
   Tactical.REVERSE (Cases_on `0 < z`) >- fs[] >>
   `x < y ∨ (x = y) ∨ y < x` by metis_tac [ordlt_trichotomy] >>
-  metis_tac [ordMULT_lt_MONO_L_EQN, ordlt_REFL]);
+  metis_tac [ordMULT_lt_MONO_R_EQN, ordlt_REFL]);
+val _ = export_rewrites ["ordMULT_CANCEL_R"]
 
 val ordMULT_continuous0 =
-  generic_continuity |> Q.INST [`f` |-> `λx. x * y`]
+  generic_continuity |> Q.INST [`f` |-> `$* a`]
                      |> SIMP_RULE (srw_ss()) []
 
 val ordMULT_continuous = store_thm(
   "ordMULT_continuous",
-  ``∀s:'a ordinal set. s ≼ univ(:'a inf) ⇒
-           (sup s * a = sup (IMAGE (λx. x * a) s))``,
+  ``∀s:'a ordinal set. s ≼ univ(:'a inf) ⇒ a * sup s = sup (IMAGE ($* a) s)``,
   rpt strip_tac >> Cases_on `s = {}` >> simp[ordMULT_continuous0]);
 
 val ordMULT_fromNat = store_thm(
   "ordMULT_fromNat",
   ``(&n : 'a ordinal) * &m = &(n * m)``,
-  Induct_on `n` >> simp[arithmeticTheory.MULT_CLAUSES]);
+  Induct_on `m` >> simp[arithmeticTheory.MULT_CLAUSES]);
 val _ = export_rewrites ["ordMULT_fromNat"]
 
 val omega_MUL_fromNat = store_thm(
   "omega_MUL_fromNat",
-  ``0 < n ⇒ ω * &n = ω``,
+  ``0 < n ⇒ &n * ω = ω``,
   simp[omax_preds_omega] >> strip_tac >>
   match_mp_tac ordle_ANTISYM >> dsimp[predimage_sup_thm, lt_omega, impI] >>
   conj_tac >- simp[ordle_lteq] >>
   qx_gen_tac `m` >>
-  qsuff_tac `&m < sup (IMAGE (λy. y * &n) (preds ω))` >- metis_tac[ordlt_REFL]>>
+  qsuff_tac `&m < sup (IMAGE ($* &n) (preds ω))` >- metis_tac[ordlt_REFL]>>
   dsimp[predimage_sup_thm, lt_omega] >>
-  qexists_tac `m + 1` >> simp[arithmeticTheory.RIGHT_ADD_DISTRIB] >>
+  qexists_tac `m + 1` >> simp[arithmeticTheory.LEFT_ADD_DISTRIB] >>
   qsuff_tac `m ≤ m * n ∧ m * n < n + m * n` >- DECIDE_TAC >>
   simp[]);
 
-val ordMULT_RDISTRIB = store_thm(
-  "ordMULT_RDISTRIB",
-  ``∀a b c:'a ordinal. (a + b) * c = a * c + b * c``,
-  qsuff_tac `∀b a c. (a + b) * c = a * c + b * c` >- simp[] >>
+val ordMULT_LDISTRIB = store_thm(
+  "ordMULT_LDISTRIB",
+  ``∀a b c:'a ordinal. c * (a + b) = c * a + c * b``,
+  qsuff_tac `∀b a c. c * (a + b) = c * a + c * b` >- simp[] >>
   ho_match_mp_tac simple_ord_induction >> simp[ordADD_ASSOC] >>
   qx_gen_tac `b` >> strip_tac >>
   `preds b ≠ {}` by (strip_tac >> fs[]) >>
@@ -1268,41 +1267,42 @@ val ordMULT_RDISTRIB = store_thm(
 val ordMULT_ASSOC = store_thm(
   "ordMULT_ASSOC",
   ``∀a b c:'a ordinal. a * (b * c) = (a * b) * c``,
-  ho_match_mp_tac simple_ord_induction >> simp[ordMULT_RDISTRIB] >>
+  qsuff_tac `∀c a b:'a ordinal. a * (b * c) = (a * b) * c` >- simp[] >>
+  ho_match_mp_tac simple_ord_induction >> simp[ordMULT_LDISTRIB] >>
   simp[ordMULT_continuous, IMAGE_cardleq_rwt, preds_inj_univ] >>
   rpt strip_tac >> AP_TERM_TAC >> dsimp[EXTENSION] >>
   asm_simp_tac (srw_ss() ++ CONJ_ss) [])
 
 val ordDIVISION0 = prove(
-  ``∀a b:'a ordinal. 0 < b ⇒ ∃q r. a = q * b + r ∧ r < b``,
+  ``∀a b:'a ordinal. 0 < b ⇒ ∃q r. a = b * q + r ∧ r < b``,
   rpt strip_tac >>
-  qabbrev_tac `d = sup { c | c * b ≤ a }` >>
-  `∀c. c * b ≤ a ⇒ c ≤ a`
+  qabbrev_tac `d = sup { c | b * c ≤ a }` >>
+  `∀c. b * c ≤ a ⇒ c ≤ a`
      by (ntac 2 strip_tac >> match_mp_tac ordle_TRANS >>
-         qexists_tac `c * b` >> simp[] >>
-         simp[Once (GSYM ordMULT_1R), SimpR ``ordlt``] >>
-         match_mp_tac ordMULT_le_MONO_R >>
+         qexists_tac `b * c` >> simp[] >>
+         match_mp_tac ordle_TRANS >> qexists_tac `1 * c` >> conj_tac >- simp[]>>
+         match_mp_tac ordMULT_le_MONO_L >>
          simp_tac bool_ss [GSYM ORD_ONE, ordlt_SUC_DISCRETE] >>
          simp[] >> strip_tac >> fs[]) >>
-  `∀α. α ∈ { c | c * b ≤ a } ⇒ α < a⁺`
+  `∀α. α ∈ { c | b * c ≤ a } ⇒ α < a⁺`
     by (simp[ordlt_SUC_DISCRETE] >> metis_tac [ordle_lteq]) >>
-  `∀α. α < d ⇔ ∃c. c * b ≤ a ∧ α < c`
+  `∀α. α < d ⇔ ∃c. b * c ≤ a ∧ α < c`
     by (simp[Abbr`d`] >> pop_assum (assume_tac o MATCH_MP ubsup_thm) >>
         simp[]) >>
-  `d * b ≤ a`
+  `b * d ≤ a`
     by (simp[Abbr`d`] >>
-        `{ c | c * b ≤ a } ≼ univ(:'a inf)`
-          by (`{ c | c * b ≤ a } ≼ preds a⁺`
+        `{ c | b * c ≤ a } ≼ univ(:'a inf)`
+          by (`{ c | b * c ≤ a } ≼ preds a⁺`
                 by simp[SUBSET_DEF, SUBSET_CARDLEQ] >>
               `preds a⁺ ≼ univ(:'a inf)` by simp[preds_inj_univ] >>
               metis_tac [cardleq_TRANS]) >>
         dsimp[ordMULT_continuous, sup_thm, IMAGE_cardleq_rwt, impI]) >>
-  `∃r. d * b + r = a` by metis_tac [ordle_EXISTS_ADD] >>
+  `∃r. b * d + r = a` by metis_tac [ordle_EXISTS_ADD] >>
   qsuff_tac `r < b` >- metis_tac[] >>
   spose_not_then strip_assume_tac >>
   `∃bb. b + bb = r` by metis_tac [ordle_EXISTS_ADD] >>
-  `d⁺ * b + bb = a` by simp[GSYM ordADD_ASSOC] >>
-  `∀c. c * b ≤ a ⇒ c ≤ d` by metis_tac [ordlt_REFL] >>
+  `b * d⁺ + bb = a` by simp[GSYM ordADD_ASSOC] >>
+  `∀c. b * c ≤ a ⇒ c ≤ d` by metis_tac [ordlt_REFL] >>
   metis_tac [ordlt_SUC, ordle_EXISTS_ADD]);
 
 val ordDIVISION = new_specification(
@@ -1317,44 +1317,44 @@ val _ = overload_on ("%", ``ordMOD``)
 
 val ordDIV_UNIQUE = store_thm(
   "ordDIV_UNIQUE",
-  ``∀a b q r. 0 < (b:'a ordinal) ∧ a = q*b + r ∧ r < b ⇒ a / b = q``,
+  ``∀a b q r. 0 < (b:'a ordinal) ∧ a = b*q + r ∧ r < b ⇒ a / b = q``,
   rpt strip_tac >>
-  `a = a / b * b + a % b ∧ a % b < b` by metis_tac [ordDIVISION] >>
+  `a = b * (a / b) + a % b ∧ a % b < b` by metis_tac [ordDIVISION] >>
   `a / b < q ∨ a / b = q ∨ q < a / b` by metis_tac [ordlt_trichotomy] >| [
     `∃bb. (q = a/b + bb) ∧ 0 < bb`
       by metis_tac [ordlt_EXISTS_ADD, ordlt_trichotomy, ordlt_ZERO] >>
-    `a = (a/b + bb) * b + r` by metis_tac[] >>
-    `_ = a/b * b + bb * b + r` by metis_tac[ordMULT_RDISTRIB] >>
-    `a % b = bb * b + r` by metis_tac [ordADD_ASSOC, ordADD_RIGHT_CANCEL] >>
-    `bb * b + r < b` by metis_tac[] >>
-    `b ≤ bb * b`
-      by (simp_tac bool_ss [Once (GSYM ordMULT_1L), SimpR ``ordlt``] >>
-          match_mp_tac ordMULT_le_MONO_L >>
+    `a = b * (a/b + bb) + r` by metis_tac[] >>
+    `_ = b * (a/b) + b * bb + r` by metis_tac[ordMULT_LDISTRIB] >>
+    `a % b = b * bb + r` by metis_tac [ordADD_ASSOC, ordADD_RIGHT_CANCEL] >>
+    `b * bb + r < b` by metis_tac[] >>
+    `b ≤ b * bb`
+      by (simp_tac bool_ss [Once (GSYM ordMULT_1R), SimpR ``ordlt``] >>
+          match_mp_tac ordMULT_le_MONO_R >>
           simp_tac bool_ss [GSYM ORD_ONE, ordlt_SUC_DISCRETE] >>
           simp[] >> strip_tac >> fs[]) >>
-    `b ≤ bb * b + r` by metis_tac [ordle_CANCEL_ADDR, ordADD_le_MONO_L,
+    `b ≤ b * bb + r` by metis_tac [ordle_CANCEL_ADDR, ordADD_le_MONO_L,
                                    ordle_TRANS],
 
     `∃bb. q + bb = a/b ∧ 0 < bb`
       by metis_tac [ordlt_EXISTS_ADD, ordlt_trichotomy, ordlt_ZERO] >>
-    `a = (q + bb) * b + a % b` by metis_tac[] >>
-    `_ = q * b + bb * b + a % b` by simp[ordMULT_RDISTRIB] >>
-    `r = bb * b + a % b` by metis_tac [ordADD_ASSOC, ordADD_RIGHT_CANCEL] >>
-    `bb * b + a % b < b` by metis_tac[] >>
-    `b ≤ bb * b`
-      by (simp_tac bool_ss [Once (GSYM ordMULT_1L), SimpR ``ordlt``] >>
-          match_mp_tac ordMULT_le_MONO_L >>
+    `a = b * (q + bb) + a % b` by metis_tac[] >>
+    `_ = b * q + b * bb + a % b` by simp[ordMULT_LDISTRIB] >>
+    `r = b * bb + a % b` by metis_tac [ordADD_ASSOC, ordADD_RIGHT_CANCEL] >>
+    `b * bb + a % b < b` by metis_tac[] >>
+    `b ≤ b * bb`
+      by (simp_tac bool_ss [Once (GSYM ordMULT_1R), SimpR ``ordlt``] >>
+          match_mp_tac ordMULT_le_MONO_R >>
           simp_tac bool_ss [GSYM ORD_ONE, ordlt_SUC_DISCRETE] >>
           simp[] >> strip_tac >> fs[]) >>
-    `b ≤ bb * b + a % b`
+    `b ≤ b * bb + a % b`
       by metis_tac [ordle_CANCEL_ADDR, ordADD_le_MONO_L, ordle_TRANS]
   ]);
 
 val ordMOD_UNIQUE = store_thm(
   "ordMOD_UNIQUE",
-  ``∀a b q r. 0 < b ∧ a = q * b + r ∧ r < b ⇒ a % b = r``,
+  ``∀a b q r. 0 < b ∧ a = b * q + r ∧ r < b ⇒ a % b = r``,
   rpt strip_tac >>
-  `(a = a / b * b + a % b) ∧ a % b < b` by metis_tac [ordDIVISION] >>
+  `(a = b * (a / b) + a % b) ∧ a % b < b` by metis_tac [ordDIVISION] >>
   `a / b = q` by metis_tac [ordDIV_UNIQUE] >> pop_assum SUBST_ALL_TAC >>
   qabbrev_tac `r' = a % b` >> fs[])
 
@@ -1363,7 +1363,7 @@ val ordEXP_def = new_specification(
   "ordEXP_def", ["ordEXP"],
   ord_RECURSION |> INST_TYPE [beta |-> ``:'a ordinal``]
                 |> Q.SPEC `1`
-                |> Q.SPEC `λap r. a * r`
+                |> Q.SPEC `λap r. r * a`
                 |> Q.SPEC `λa preds. sup preds`
                 |> Q.GEN `a`
                 |> CONV_RULE SKOLEM_CONV
@@ -1372,7 +1372,6 @@ val ordEXP_def = new_specification(
 val _ = export_rewrites ["ordEXP_def"]
 val _ = overload_on ("**", ``ordEXP``)
 
-val _ = export_rewrites ["ordMULT_1R"]
 val ordEXP_1R = store_thm(
   "ordEXP_1R",
   ``(a:'a ordinal) ** 1 = a``,
@@ -1404,7 +1403,7 @@ val ordEXP_le_MONO_L = store_thm(
   ho_match_mp_tac simple_ord_induction >> simp[] >> conj_tac
   >- (qx_gen_tac `x` >> strip_tac >> map_every qx_gen_tac [`a`, `b`] >>
       strip_tac >> match_mp_tac ordle_TRANS >>
-      qexists_tac `b * a ** x` >> simp[ordMULT_le_MONO_L, ordMULT_le_MONO_R]) >>
+      qexists_tac `a ** x * b` >> simp[ordMULT_le_MONO_L, ordMULT_le_MONO_R]) >>
   qx_gen_tac `x` >> strip_tac >> map_every qx_gen_tac [`a`, `b`] >>
   strip_tac >> simp[predimage_sup_thm, impI] >>
   qx_gen_tac `d` >> strip_tac >>
@@ -1459,7 +1458,7 @@ val ordEXP_ZERO_nonlimit = store_thm(
   "ordEXP_ZERO_nonlimit",
   ``¬islimit x ⇒ 0 ** x = 0``,
   metis_tac [preds_omax_SOME_SUC, optionTheory.option_CASES, ordEXP_def,
-             ordMULT_def]);
+             ordMULT_0R]);
 
 val sup_EQ_0 = store_thm(
   "sup_EQ_0",
@@ -1490,6 +1489,7 @@ val IMAGE_EQ_SING = store_thm(
 val ordMULT_EQ_0 = store_thm(
   "ordMULT_EQ_0",
   ``∀x y. x * y = 0 ⇔ x = 0 ∨ y = 0``,
+  CONV_TAC SWAP_FORALL_CONV >>
   ho_match_mp_tac simple_ord_induction >> simp[] >>
   simp_tac (srw_ss() ++ CONJ_ss) [] >> qx_gen_tac `x` >> strip_tac >>
   simp[sup_EQ_0, IMAGE_cardleq_rwt, preds_inj_univ] >>
@@ -1531,7 +1531,7 @@ val ordEXP_lt_MONO_R = store_thm(
   >- (simp[ordlt_SUC_DISCRETE] >> rw[] >| [
         match_mp_tac ordlt_TRANS >> qexists_tac `a ** y` >> simp[],
         ALL_TAC
-      ] >> simp_tac bool_ss [SimpL ``ordlt``, Once (GSYM ordMULT_1L)] >>
+      ] >> simp_tac bool_ss [SimpL ``ordlt``, Once (GSYM ordMULT_1R)] >>
       simp[ZERO_lt_ordEXP] >> DISJ1_TAC >>
       match_mp_tac ordlt_TRANS >> qexists_tac `1` >> simp[]) >>
   simp[predimage_sup_thm] >> fs[omax_NONE] >>
@@ -1562,7 +1562,7 @@ val ordEXP_continuous = store_thm(
 
 val ordEXP_ADD = store_thm(
   "ordEXP_ADD",
-  ``0 < x ⇒ x ** (y + z) = x ** z * x ** y``,
+  ``0 < x ⇒ x ** (y + z) = x ** y * x ** z``,
   map_every qid_spec_tac [`x`,`y`,`z`] >>
   ho_match_mp_tac simple_ord_induction >> simp[ordMULT_ASSOC] >>
   qx_gen_tac `z` >> strip_tac >> map_every qx_gen_tac [`y`, `x`] >>
@@ -1574,7 +1574,7 @@ val ordEXP_ADD = store_thm(
 
 val ordEXP_MUL = store_thm(
   "ordEXP_MUL",
-  ``0 < x ⇒ x ** (z * y) = (x ** y) ** z``,
+  ``0 < x ⇒ x ** (y * z) = (x ** y) ** z``,
   strip_tac >> map_every qid_spec_tac [`y`, `z`] >>
   ho_match_mp_tac simple_ord_induction >> simp[ordEXP_ADD] >>
   qx_gen_tac `z` >> strip_tac >> qx_gen_tac `y` >>
@@ -1622,12 +1622,12 @@ val x_le_ordEXP_x = store_thm(
   gen_tac >> Cases_on `1 < a` >> simp[] >>
   ho_match_mp_tac simple_ord_induction >> simp[] >> conj_tac >>
   qx_gen_tac `x` >> strip_tac
-  >- (qsuff_tac `x < a * a ** x`
+  >- (qsuff_tac `x < a ** x * a`
       >- (simp[ordlt_SUC_DISCRETE] >> simp[ordle_lteq] >>
           metis_tac[ordlt_REFL]) >>
-      qsuff_tac `a ** x < a * a ** x`
+      qsuff_tac `a ** x < a ** x * a`
       >- metis_tac[ordle_lteq, ordlt_TRANS] >>
-      SIMP_TAC bool_ss [SimpL ``ordlt``, Once (GSYM ordMULT_1L)] >>
+      SIMP_TAC bool_ss [SimpL ``ordlt``, Once (GSYM ordMULT_1R)] >>
       simp[ZERO_lt_ordEXP] >> DISJ1_TAC >> match_mp_tac ordlt_TRANS >>
       qexists_tac `1` >> simp[]) >>
   `∀b. b < x ⇒ b⁺ < x` by metis_tac [islimit_SUC_lt] >>
@@ -1715,26 +1715,26 @@ val add_omega_islimit = store_thm(
   simp[omax_preds_omega, ordADD_continuous])
 val _ = export_rewrites ["add_omega_islimit"]
 
-val islimit_mul_L = store_thm(
-  "islimit_mul_L",
-  ``∀α. islimit α ⇒ islimit (α * β)``,
+val islimit_mul_R = store_thm(
+  "islimit_mul_R",
+  ``∀α. islimit α ⇒ islimit (β * α)``,
   Cases_on `β = 0` >- simp[] >> fs[IFF_ZERO_lt] >> gen_tac >>
   Cases_on `α = 0` >- simp[] >> fs[IFF_ZERO_lt] >> strip_tac >>
-  qspec_then `λx. x * β` mp_tac
+  qspec_then `$* β` mp_tac
     (Q.GEN `f` strict_continuity_preserves_islimit) >> simp[] >>
   simp[ordMULT_continuous, IFF_ZERO_lt])
 
 val mul_omega_islimit = store_thm(
   "mul_omega_islimit",
-  ``islimit (α * ω)``,
-  qspec_then `α` strip_assume_tac ord_CASES >> simp[islimit_mul_L]);
+  ``islimit (ω * α)``,
+  qspec_then `α` strip_assume_tac ord_CASES >> simp[islimit_mul_R]);
 
 val omega_exp_islimit = store_thm(
   "omega_exp_islimit",
   ``0 < α ⇒ islimit (ω ** α)``,
   qspec_then `α` strip_assume_tac ord_CASES
   >- simp[]
-  >- (simp[] >> simp[islimit_mul_L, omax_preds_omega]) >>
+  >- (simp[] >> simp[islimit_mul_R, omax_preds_omega]) >>
   strip_tac >> ho_match_mp_tac strict_continuity_preserves_islimit >>
   simp[IFF_ZERO_lt, ordEXP_continuous]);
 
@@ -1752,10 +1752,10 @@ val expbound_add = store_thm(
       disch_then (CONJUNCTS_THEN2
                   (Q.X_CHOOSE_THEN `b` strip_assume_tac)
                   (Q.X_CHOOSE_THEN `c` strip_assume_tac)) >>
-      `x + y < &(b + c) * ω ** a`
-        by (simp_tac bool_ss [ordMULT_RDISTRIB, GSYM ordADD_fromNat] >>
+      `x + y < ω ** a * &(b + c)`
+        by (simp_tac bool_ss [ordMULT_LDISTRIB, GSYM ordADD_fromNat] >>
             match_mp_tac ordlte_TRANS >>
-            qexists_tac `x + &c * ω ** a` >> simp[] >>
+            qexists_tac `x + ω ** a * &c` >> simp[] >>
             simp[ordADD_weak_MONO]) >>
       asm_simp_tac(srw_ss() ++ DNF_ss)[] >> qexists_tac `&(b + c)` >>
       simp[]) >>
@@ -1787,11 +1787,11 @@ val ordMUL_under_epsilon0 = store_thm(
   strip_tac >> imp_res_tac epsilon0_least_fixpoint >>
   `x * y < ω ** x * ω ** y`
     by (match_mp_tac ordlet_TRANS >>
-        qexists_tac `x * ω ** y` >> simp[ZERO_lt_ordEXP] >>
-        match_mp_tac ordMULT_le_MONO_R >> simp[ordle_lteq]) >>
-  `ω ** x * ω ** y = ω ** (y + x)` by simp[ordEXP_ADD] >>
+        qexists_tac `ω ** x * y` >> simp[ZERO_lt_ordEXP] >>
+        match_mp_tac ordMULT_le_MONO_L >> simp[ordle_lteq]) >>
+  `ω ** x * ω ** y = ω ** (x + y)` by simp[ordEXP_ADD] >>
   pop_assum SUBST_ALL_TAC >>
-  qsuff_tac `ω ** (y + x) < ε₀` >- metis_tac[ordlt_TRANS] >>
+  qsuff_tac `ω ** (x + y) < ε₀` >- metis_tac[ordlt_TRANS] >>
   metis_tac [epsilon0_fixpoint, ordADD_under_epsilon0, fromNat_lt_omega,
              ordEXP_lt_IFF]);
 
@@ -1801,22 +1801,16 @@ val ordEXP_under_epsilon0 = store_thm(
   strip_tac >>
   `a < ω ** a` by imp_res_tac epsilon0_least_fixpoint >>
   `a ** b <= (ω ** a) ** b` by metis_tac [ordEXP_le_MONO_L, ordle_lteq] >>
-  `(ω ** a) ** b = ω ** (b * a)` by simp [GSYM ordEXP_MUL] >>
+  `(ω ** a) ** b = ω ** (a * b)` by simp [GSYM ordEXP_MUL] >>
   pop_assum SUBST_ALL_TAC >>
-  `ω ** (b * a) < ε₀`
+  `ω ** (a * b) < ε₀`
     by simp[ordEXP_lt_IFF, ordMUL_under_epsilon0,
             Once (GSYM epsilon0_fixpoint)] >>
   metis_tac [ordlet_TRANS]);
 
-val FOLDL_SUM_lemma = prove(
-  ``∀ces x s:'a ordinal.
-       x + FOLDL (λacc (c,e). acc + c * a ** e) s ces =
-       FOLDL (λacc (c,e). acc + c * a ** e) (x + s) ces``,
-  Induct >> simp[pairTheory.FORALL_PROD] >> simp[ordADD_ASSOC]);
-
 val eval_poly_def = Define`
   eval_poly (a:'a ordinal) [] = 0 ∧
-  eval_poly a ((c,e)::t) = c * a ** e + eval_poly a t
+  eval_poly a ((c,e)::t) = a ** e * c + eval_poly a t
 `;
 val _ = export_rewrites ["eval_poly_def"]
 
@@ -1884,13 +1878,13 @@ val polyform_exists = store_thm(
   qabbrev_tac `c1 = b / a ** E` >>
   qabbrev_tac `r = b % a ** E` >>
   `0 < a ** E` by simp[ZERO_lt_ordEXP] >>
-  `b = c1 * a ** E + r ∧ r < a ** E` by metis_tac [ordDIVISION] >>
+  `b = a ** E * c1 + r ∧ r < a ** E` by metis_tac [ordDIVISION] >>
   `r < b` by metis_tac [ordlt_TRANS, ordle_lteq] >>
   `0 < c1` by (spose_not_then strip_assume_tac >> fs[]) >>
   `c1 < a`
     by (spose_not_then strip_assume_tac >>
-        `a * a ** E ≤ c1 * a ** E` by simp[] >>
-        `a * a ** E + r ≤ b` by simp[ordADD_le_MONO_L] >>
+        `a ** E * a ≤ a ** E * c1` by simp[] >>
+        `a ** E * a + r ≤ b` by simp[ordADD_le_MONO_L] >>
         metis_tac [ordEXP_def, ordle_CANCEL_ADDR, ordle_TRANS]) >>
   `∃ces. (∀i j. i < j ∧ j < LENGTH ces ⇒ SND (EL j ces) < SND (EL i ces)) ∧
          (∀c e. MEM (c,e) ces ⇒ 0 < c ∧ c < a) ∧
@@ -1912,12 +1906,12 @@ val polyform_exists = store_thm(
   `ces = [] ∨ ∃c0 e0 t. ces = (c0,e0)::t`
     by metis_tac [pairTheory.pair_CASES, listTheory.list_CASES] >- simp[] >>
   simp[] >> (* rts: e0 < E *) spose_not_then strip_assume_tac >>
-  `r = c0 * a ** e0 + eval_poly a t` by simp[] >>
+  `r = a ** e0 * c0 + eval_poly a t` by simp[] >>
   `a ** E ≤ a ** e0` by simp[ordEXP_le_MONO_R] >>
-  `a ** e0 ≤ c0 * a ** e0`
-    by (simp_tac bool_ss [SimpR ``ordlt``, Once (GSYM ordMULT_1L)] >>
-        match_mp_tac ordMULT_le_MONO_L >> simp[IFF_ZERO_lt] >> fs[]) >>
-  `c0 * a ** e0 ≤ c0 * a ** e0 + eval_poly a t` by simp[] >>
+  `a ** e0 ≤ a ** e0 * c0`
+    by (simp_tac bool_ss [SimpR ``ordlt``, Once (GSYM ordMULT_1R)] >>
+        match_mp_tac ordMULT_le_MONO_R >> simp[IFF_ZERO_lt] >> fs[]) >>
+  `a ** e0 * c0 ≤ a ** e0 * c0 + eval_poly a t` by simp[] >>
   metis_tac [ordle_TRANS, ordle_lteq, ordlt_REFL, ordlt_TRANS])
 
 val polyform_def = new_specification(
@@ -1942,9 +1936,9 @@ val polyform_0 = store_thm(
     by metis_tac[pairTheory.pair_CASES, listTheory.list_CASES]
     >- simp[] >>
   simp[SimpL ``$==>``] >> strip_tac >> fs[]
-  >- (`0 < c` by metis_tac[is_polyform_ELthm,listTheory.MEM] >>
-      metis_tac[IFF_ZERO_lt]) >>
-  fs[ordEXP_EQ_0]);
+  >- fs[ordEXP_EQ_0] >>
+  `0 < c` by metis_tac[is_polyform_ELthm,listTheory.MEM] >>
+  metis_tac[IFF_ZERO_lt]);
 
 val polyform_EQ_NIL = store_thm(
   "polyform_EQ_NIL",
@@ -1961,13 +1955,14 @@ val is_polyform_CONS_E = store_thm(
 
 val expbounds = prove(
   ``1 < (a:'a ordinal) ∧ y < a ** e ∧ c < a ∧ e < e' ⇒
-    c * a ** e + y < a ** e'``,
+    a ** e * c + y < a ** e'``,
   strip_tac >>
-  `c * a ** e + y < c * a ** e + a ** e` by simp[] >>
-  `c * a ** e + a ** e = c⁺ * a ** e` by simp[] >> pop_assum SUBST_ALL_TAC >>
+  `a ** e * c + y < a ** e * c + a ** e` by simp[] >>
+  `a ** e * c + a ** e = a ** e * ordSUC c` by simp[] >>
+  pop_assum SUBST_ALL_TAC >>
   `c⁺ ≤ a` by metis_tac [ordlt_DISCRETE1] >>
-  `c⁺ * a ** e ≤ a * a ** e` by simp[ordMULT_le_MONO_L] >>
-  `a * a ** e = a ** e⁺` by simp[] >> pop_assum SUBST_ALL_TAC >>
+  `a ** e * c⁺ ≤ a ** e * a` by simp[ordMULT_le_MONO_R] >>
+  `a ** e * a = a ** e⁺` by simp[] >> pop_assum SUBST_ALL_TAC >>
   `a ** e⁺ ≤ a ** e'`
      by (match_mp_tac ordEXP_le_MONO_R >> conj_tac
          >- (spose_not_then strip_assume_tac >> fs[]) >>
@@ -1989,34 +1984,34 @@ val is_polyform_head_dominates_tail = store_thm(
 
 val cx_lt_x = store_thm(
   "cx_lt_x",
-  ``c * x < (x:'a ordinal) ⇔ 0 < x ∧ c = 0``,
-  simp_tac bool_ss [SimpLHS, SimpR ``ordlt``, Once (GSYM ordMULT_1L)] >>
+  ``x * c < (x:'a ordinal) ⇔ 0 < x ∧ c = 0``,
+  simp_tac bool_ss [SimpLHS, SimpR ``ordlt``, Once (GSYM ordMULT_1R)] >>
   simp[] >> metis_tac [IFF_ZERO_lt]);
 val _ = export_rewrites ["cx_lt_x"]
 
 val explemma = prove(
-  ``1 < a ∧ c1 * a ** e1 + eval_poly a t1 = c2 * a ** e2 + eval_poly a t2 ∧
+  ``1 < a ∧ a ** e1 * c1 + eval_poly a t1 = a ** e2 * c2 + eval_poly a t2 ∧
     is_polyform a ((c1,e1)::t1) ∧ is_polyform a ((c2,e2)::t2) ⇒
     e1 ≤ e2``,
   rpt strip_tac (* e2 < e1 *) >>
   `eval_poly a t2 < a ** e2` by metis_tac [is_polyform_head_dominates_tail] >>
   imp_res_tac is_polyform_CONS_E >>
-  `c2 * a ** e2 + eval_poly a t2 < a ** e1` by simp[expbounds] >>
-  `a ** e1 ≤ c1 * a ** e1` by simp[IFF_ZERO_lt] >>
-  `c1 * a ** e1 ≤ c1 * a ** e1 + eval_poly a t1` by simp[] >>
+  `a ** e2 * c2 + eval_poly a t2 < a ** e1` by simp[expbounds] >>
+  `a ** e1 ≤ a ** e1 * c1` by simp[IFF_ZERO_lt] >>
+  `a ** e1 * c1 ≤ a ** e1 * c1 + eval_poly a t1` by simp[] >>
   metis_tac[ordlte_TRANS, ordle_TRANS, ordlt_REFL]);
 
 val coefflemma = prove(
-  ``1 < a ∧ c1 * a ** e + eval_poly a t1 = c2 * a ** e + eval_poly a t2 ∧
+  ``1 < a ∧ a ** e * c1 + eval_poly a t1 = a ** e * c2 + eval_poly a t2 ∧
     is_polyform a ((c1,e)::t1) ∧ is_polyform a ((c2,e)::t2) ⇒
     c1 ≤ c2``,
   rpt strip_tac (* c2 < c1 *) >>
   `eval_poly a t2 < a ** e` by metis_tac [is_polyform_head_dominates_tail] >>
   imp_res_tac is_polyform_CONS_E >>
-  `c2 * a ** e + eval_poly a t2 < c2 * a ** e + a ** e` by simp[] >>
-  `c2 * a ** e + a ** e = c2⁺ * a ** e` by simp[] >> pop_assum SUBST_ALL_TAC >>
-  `c2⁺ * a ** e ≤ c1 * a ** e` by (simp[] >> metis_tac [ordlt_DISCRETE1]) >>
-  `c1 * a ** e ≤ c1 * a ** e + eval_poly a t1` by simp[] >>
+  `a ** e * c2 + eval_poly a t2 < a ** e * c2 + a ** e` by simp[] >>
+  `a ** e * c2 + a ** e = a ** e * c2⁺` by simp[] >> pop_assum SUBST_ALL_TAC >>
+  `a ** e * c2⁺ ≤ a ** e * c1` by (simp[] >> metis_tac [ordlt_DISCRETE1]) >>
+  `a ** e * c1 ≤ a ** e * c1 + eval_poly a t1` by simp[] >>
   metis_tac [ordlte_TRANS, ordle_TRANS, ordlt_REFL]);
 
 val polyform_UNIQUE = store_thm(
@@ -2034,12 +2029,12 @@ val polyform_UNIQUE = store_thm(
   >- (pop_assum SUBST_ALL_TAC >> `b = 0` by fs[] >> simp[polyform_0]) >>
   pop_assum SUBST_ALL_TAC >>
   `0 < c ∧ c < a` by metis_tac[listTheory.MEM, is_polyform_ELthm] >>
-  `b = c * a ** e + eval_poly a t` by fs[] >>
+  `b = a ** e * c + eval_poly a t` by fs[] >>
   `polyform a b ≠ []` by simp[polyform_EQ_NIL, IFF_ZERO_lt, ZERO_lt_ordEXP] >>
   `∃c' e' t'. polyform a b = (c',e')::t'`
     by metis_tac [listTheory.list_CASES, pairTheory.pair_CASES] >>
   `0 < c' ∧ c' < a` by metis_tac [is_polyform_CONS_E] >>
-  `b = c' * a ** e' + eval_poly a t'` by fs[] >>
+  `b = a ** e' * c' + eval_poly a t'` by fs[] >>
   `e' = e` by metis_tac [explemma, ordle_ANTISYM] >> pop_assum SUBST_ALL_TAC >>
   `c' = c` by metis_tac [coefflemma, ordle_ANTISYM] >> pop_assum SUBST_ALL_TAC>>
   `eval_poly a t = eval_poly a t'` by metis_tac [ordADD_RIGHT_CANCEL] >>
@@ -2047,8 +2042,8 @@ val polyform_UNIQUE = store_thm(
   `eval_poly a t < b`
     by (`eval_poly a t < a ** e`
           by metis_tac [is_polyform_head_dominates_tail] >>
-        `a ** e ≤ c * a ** e` by simp[IFF_ZERO_lt] >>
-        `c * a ** e ≤ c * a ** e + eval_poly a t` by simp[] >>
+        `a ** e ≤ a ** e * c` by simp[IFF_ZERO_lt] >>
+        `a ** e * c ≤ a ** e * c + eval_poly a t` by simp[] >>
         metis_tac [ordlte_TRANS, ordle_TRANS]) >>
   metis_tac [is_polyform_CONS_E]);
 
